formalization/Typing.v
@@ -28,11 +28,19 @@ Inductive wf_pty: listctx pty -> pty -> Prop :=
     closed_pty (ctxdom ⦑ Γ ⦒) {v: b | ϕ } -> wf_pty Γ {v: b | ϕ }
 | wf_pty_arr: forall Γ ρ T A B (L: aset),
     wf_pty Γ ρ ->
-    wf_am Γ A ->
     amlist_typed B T ->
+    (* NOTE: we do not allow empty union here; it does not affect
+    expressiveness, as we can always use [aemp] instead. *)
+    B <> [] ->
+    (forall x, x ∉ L ->
+          wf_am (Γ ++ [(x, ρ)]) (A ^a^ x) /\
+          (forall Bi ρi, In (Bi, ρi) B ->
+                    wf_am (Γ ++ [(x, ρ)]) (Bi ^a^ x)
+          )
+    ) ->
     (forall x, x ∉ L ->
           (forall Bi ρi, In (Bi, ρi) B ->
-                    wf_pty (Γ ++ [(x, ρ)]) ρi
+                    wf_pty (Γ ++ [(x, ρ)]) (ρi ^p^ x)
           )
     ) ->
     wf_pty Γ (-: ρ ⤑[: T | A ⇒ B ]).
@@ -40,7 +48,9 @@ Inductive wf_pty: listctx pty -> pty -> Prop :=
 Inductive wf_hty: listctx pty -> hty -> Prop :=
 | wf_hty_: forall Γ T A B,
     amlist_typed B T ->
-    (forall Ai ρi, In (Ai, ρi) B -> wf_am Γ Ai /\ wf_pty Γ ρi) ->
+    B <> [] ->
+    wf_am Γ A ->
+    (forall Bi ρi, In (Bi, ρi) B -> wf_am Γ Bi /\ wf_pty Γ ρi) ->
     wf_hty Γ [: T | A ⇒ B ].
 
 Notation " Γ '⊢WF' τ " := (wf_hty Γ τ) (at level 20, τ constr, Γ constr).
@@ -48,6 +58,7 @@ Notation " Γ '⊢WFp' τ " := (wf_pty Γ τ) (at level 20, τ constr, Γ constr
 
 Definition subtyping (Γ: listctx pty) (τ1 τ2: hty) : Prop :=
   (* Assume [τ1] and [τ2] are valid [hty]s. *)
+  ⌊ τ1 ⌋ = ⌊ τ2 ⌋ /\
   forall Γv, ctxRst Γ Γv -> forall e, ⟦(m{ Γv }h) τ1⟧ (m{ Γv }t e) → ⟦(m{ Γv }h) τ2⟧ (m{ Γv }t e).
 
 Notation " Γ '⊢' τ1 '⪡' τ2 " := (subtyping Γ τ1 τ2) (at level 20, τ1 constr, τ2 constr, Γ constr).
@@ -69,35 +80,42 @@ Inductive term_type_check : listctx pty -> tm -> hty -> Prop :=
 | TLetE: forall Γ e_x e Tx A T Bx_ρx BxB_ρ Bx_ρx_B_ρ (L: aset),
     Γ ⊢WF [: T | A ⇒ BxB_ρ ] ->
     Γ ⊢ e_x ⋮t [: Tx | A ⇒ Bx_ρx ] ->
-    Bx_ρx = map (fun '(Bx, ρx, _, _) => (Bx, ρx)) Bx_ρx_B_ρ ->
-    BxB_ρ = map (fun '(Bx, _, B, ρ) => (aconcat Bx B, ρ)) Bx_ρx_B_ρ ->
+    Forall2 (fun '(Bx, ρx) '(Bx', ρx', _, _) =>
+               Bx = Bx' /\ ρx = ρx') Bx_ρx Bx_ρx_B_ρ ->
+    Forall2 (fun '(BxB, ρ) '(Bx, _, B, ρ') =>
+               BxB = aconcat Bx B /\ ρ = ρ') BxB_ρ Bx_ρx_B_ρ ->
     (forall x, x ∉ L ->
           forall Bxi ρxi Bi ρi,
             In (Bxi, ρxi, Bi, ρi) Bx_ρx_B_ρ ->
             (Γ ++ [(x, ρxi)]) ⊢ (e ^t^ x) ⋮t [: T | aconcat A Bxi ⇒ [(Bi, ρi)]]) ->
     Γ ⊢ (tlete e_x e) ⋮t [: T | A ⇒ BxB_ρ ]
 | TApp: forall Γ (v1 v2: value) e ρ Tx A T Bx_ρx BxB_ρ Bx_ρx_B_ρ (L: aset),
-    Γ ⊢WF [: T | A ⇒ BxB_ρ ] ->
+    Γ ⊢WF [: T | A ^a^ v2 ⇒ BxB_ρ ] ->
     Γ ⊢ v2 ⋮v ρ ->
     Γ ⊢ v1 ⋮v (-: ρ ⤑[: Tx | A ⇒ Bx_ρx ]) ->
-    Bx_ρx = map (fun '(Bx, ρx, _, _) => (Bx, ρx)) Bx_ρx_B_ρ ->
-    BxB_ρ = map (fun '(Bx, _, B, ρ) => (aconcat Bx B, ρ)) Bx_ρx_B_ρ ->
+    Forall2 (fun '(Bx, ρx) '(Bx', ρx', _, _) =>
+               Bx = Bx' /\ ρx = ρx') Bx_ρx Bx_ρx_B_ρ ->
+    Forall2 (fun '(BxB, ρ) '(Bx, _, B, ρ') =>
+               BxB = aconcat (Bx ^a^ v2) B /\ ρ = ρ') BxB_ρ Bx_ρx_B_ρ ->
     (forall x, x ∉ L ->
           forall Bxi ρxi Bi ρi,
             In (Bxi, ρxi, Bi, ρi) Bx_ρx_B_ρ ->
-            (Γ ++ [(x, ρxi ^p^ v2)]) ⊢ (e ^t^ x) ⋮t [: T | aconcat A (Bxi ^a^ v2) ⇒ [(Bi, ρi)]]) ->
-    Γ ⊢ (tletapp v1 v2 e) ⋮t [: T | A ⇒ BxB_ρ ]
-| TEffOp: forall Γ (op: effop) (v2: value) e ρ A ϕx T Aop' Bi ρi (L: aset),
-    (* NOTE: it does not seem like we need to substitute [ϕx] here, i.e. [{1 ~q>
-    v2}ϕx], because bound variable [1] is already restricted to [v2]. *)
-    Aop' = ⟨ op | b1:v= v2 & ϕx ⟩ ->
-    Γ ⊢WF [: T | A ^a^ v2 ⇒ [(aconcat Aop' Bi, ρi)] ] ->
-    builtin_typing_relation op (-: ρ ⤑[: ret_ty_of_op op | A ⇒ [(aϵ, {v: ret_ty_of_op op | ϕx})] ]) ->
+            (Γ ++ [(x, ρxi ^p^ v2)]) ⊢ (e ^t^ x) ⋮t [: T | aconcat (A ^a^ v2) (Bxi ^a^ v2) ⇒ [(Bi, ρi)]]) ->
+    Γ ⊢ (tletapp v1 v2 e) ⋮t [: T | A ^a^ v2 ⇒ BxB_ρ ]
+| TEffOp: forall Γ (op: effop) (v2: value) e ρ ρx A T Bx_ρx opϕB_ρ ϕ_B_ρ (L: aset),
+    Γ ⊢WF [: T | A ^a^ v2 ⇒ opϕB_ρ ] ->
     Γ ⊢ v2 ⋮v ρ ->
+    builtin_typing_relation op ρx ->
+    Γ ⊢ pty_to_rty ρx ⪡ pty_to_rty (-: ρ ⤑[: ret_ty_of_op op | A ⇒ Bx_ρx]) ->
+    Forall2 (fun '(Bx, ρx) '(ϕ, _, _) =>
+               Bx = aϵ /\ ρx = {v: ret_ty_of_op op | ϕ}) Bx_ρx ϕ_B_ρ ->
+    Forall2 (fun '(opϕB, ρ) '(ϕ, B, ρ') =>
+               opϕB = aconcat (⟨ op | b1:v= v2 & ϕ ⟩) B /\ ρ = ρ') opϕB_ρ ϕ_B_ρ ->
     (forall x, x ∉ L ->
-          forall Aop, Aop = ⟨ op | b1:v= v2 & b0:x= x ⟩ ->
-          (Γ ++ [(x, {v: ret_ty_of_op op | {1 ~q> v2 } ϕx})]) ⊢ (e ^t^ x) ⋮t ([: T | aconcat A Aop ⇒ [(Bi, ρi)]] ^h^ x)) ->
-    Γ ⊢ (tleteffop op v2 e) ⋮t [: T | A ^a^ v2 ⇒ [(aconcat Aop' Bi, ρi)] ]
+          forall ϕi Bi ρi,
+            In (ϕi, Bi, ρi) ϕ_B_ρ ->
+            (Γ ++ [(x, {v: ret_ty_of_op op | {1 ~q> v2} ϕi})]) ⊢ (e ^t^ x) ⋮t [: T | aconcat (A ^a^ v2) (⟨ op | b1:v= v2 & b0:x= x ⟩) ⇒ [(Bi, ρi)]]) ->
+    Γ ⊢ (tleteffop op v2 e) ⋮t [: T | A ^a^ v2 ⇒ opϕB_ρ ]
 | TMatchb_true: forall Γ (v: value) e1 e2 τ,
     Γ ⊢WF τ ->
     Γ ⊢ v ⋮v (mk_eq_constant true) ->
@@ -115,15 +133,18 @@ with value_type_check : listctx pty -> value -> pty -> Prop :=
     Γ ⊢WFp (mk_eq_constant c) ->
     Γ ⊢ c ⋮v (mk_eq_constant c)
 | TVar: forall Γ (x: atom) ρ,
+    Γ ⊢WFp ρ ->
     ctxfind Γ x = Some ρ ->
     Γ ⊢ x ⋮v ρ
 | TLam: forall Γ Tx ρ e T A B (L: aset),
     Γ ⊢WFp (-: ρ ⤑[: T | A ⇒ B ] ) ->
     (forall x, x ∉ L -> (Γ ++ [(x, ρ)]) ⊢ (e ^t^ x) ⋮t ([: T | A ⇒ B ] ^h^ x)) ->
+    Tx = ⌊ ρ ⌋ ->
     Γ ⊢ (vlam Tx e) ⋮v (-: ρ ⤑[: T | A ⇒ B ])
-| TLamFix: forall Γ Tx ρ e T A B (L: aset),
+| TLamFix: forall Γ (Tx : base_ty) ρ e T A B (L: aset),
     Γ ⊢WFp (-: ρ ⤑[: T | A ⇒ B ]) ->
     (forall f, f ∉ L -> (Γ ++ [(f, (-: ρ ⤑[: T | A ⇒ B ]))]) ⊢ ((vlam Tx e) ^v^ f) ⋮v (-: ρ ⤑[: T | A ⇒ B ])) ->
+    TBase Tx = ⌊ ρ ⌋ ->
     Γ ⊢ (vfix (⌊ -: ρ ⤑[: T | A ⇒ B ] ⌋) (vlam Tx e)) ⋮v (-: ρ ⤑[: T | A ⇒ B ])
 where
 "Γ '⊢' e '⋮t' τ" := (term_type_check Γ e τ) and "Γ '⊢' e '⋮v' τ" := (value_type_check Γ e τ).
@@ -132,13 +153,81 @@ where
 Scheme value_type_check_rec := Induction for value_type_check Sort Prop
     with term_type_check_rec := Induction for term_type_check Sort Prop.
 
-Lemma value_typing_regular: forall (Γ: listctx pty) (v: value) (ρ: pty),
-    Γ ⊢ v ⋮v ρ -> ⌊ Γ ⌋* ⊢t v ⋮v ⌊ ρ ⌋ /\ wf_pty Γ ρ.
-Admitted.
+Lemma pty_to_rty_wf Γ ρ :
+  wf_pty Γ ρ ->
+  wf_hty Γ (pty_to_rty ρ).
+Proof.
+  unfold pty_to_rty.
+  induction 1.
+  - cbn. econstructor.
+    hnf. intros. qauto. eauto.
+    repeat econstructor. my_set_solver.
+    qsimpl. repeat econstructor. my_set_solver.
+  - cbn. econstructor.
+    hnf. intros. qauto. eauto.
+    repeat econstructor. my_set_solver.
+    qsimpl.
+Qed.
 
-Lemma tm_typing_regular: forall (Γ: listctx pty) (e: tm) (τ: hty),
-    Γ ⊢ e ⋮t τ -> ⌊ Γ ⌋* ⊢t e ⋮t ⌊ τ ⌋ /\ wf_hty Γ τ.
-Admitted.
+Lemma subtyping_preserves_basic_typing Γ τ1 τ2 :
+  Γ ⊢ τ1 ⪡ τ2 ->
+  ⌊τ1⌋ = ⌊τ2⌋.
+Proof.
+  qauto.
+Qed.
+
+Lemma value_typing_regular_wf : forall (Γ: listctx pty) (v: value) (ρ: pty),
+    Γ ⊢ v ⋮v ρ -> wf_pty Γ ρ
+with tm_typing_regular_wf : forall (Γ: listctx pty) (e: tm) (τ: hty),
+    Γ ⊢ e ⋮t τ -> wf_hty Γ τ.
+Proof.
+  all: destruct 1; eauto using pty_to_rty_wf.
+Qed.
+
+(* Maybe move these lemmas to other files. *)
+Lemma list_not_nil_ex {A} (xs : list A) :
+  xs <> [] ->
+  exists x, In x xs.
+Proof.
+  destruct xs; qauto.
+Qed.
+
+Lemma Forall2_In_l {A B} R (xs : list A) (ys : list B) :
+  Forall2 R xs ys ->
+  forall x, In x xs -> exists y, In y ys /\ R x y.
+Proof.
+  induction 1; qauto.
+Qed.
+
+Lemma Forall2_In_r {A B} R (xs : list A) (ys : list B) :
+  Forall2 R xs ys ->
+  forall y, In y ys -> exists x, In x xs /\ R x y.
+Proof.
+  induction 1; qauto.
+Qed.
+
+Ltac simpl_Forall2 :=
+  repeat
+    (match goal with
+     | H : _ <> [] |- _ => apply list_not_nil_ex in H
+     | H : Forall2 _ ?xs _, H' : In _ ?xs |- _ =>
+         eapply Forall2_In_l in H; [ | apply H' ]
+     | H : Forall2 _ _ ?ys, H' : In _ ?ys |- _ =>
+         eapply Forall2_In_r in H; [ | apply H' ]
+     end; simp_hyps; simplify_eq); set_fold_not.
+
+Lemma union_list_subseteq_forall
+  {A C} `{SemiSet A C}
+  (xs : list C) (s : C):
+  (forall x, In x xs -> x ⊆ s) ->
+  ⋃ xs ⊆ s.
+Proof.
+  intros. induction xs. my_set_solver.
+  simpl.
+  apply union_least.
+  qauto.
+  qauto.
+Qed.
 
 Lemma well_formed_builtin_typing: forall op ρx A B ρ,
     builtin_typing_relation op (-: ρx ⤑[: ret_ty_of_op op | A ⇒ [(B, ρ)] ]) ->
@@ -148,51 +237,53 @@ Lemma well_formed_builtin_typing: forall op ρx A B ρ,
                               (forall (c: constant), α ⊧{op ~ v_x}⇓{ c } -> p⟦ ρ ^p^ v_x ⟧ c).
 Admitted.
 
+Lemma value_typing_regular_basic_typing: forall (Γ: listctx pty) (v: value) (ρ: pty),
+    Γ ⊢ v ⋮v ρ -> ⌊ Γ ⌋* ⊢t v ⋮v ⌊ ρ ⌋
+with tm_typing_regular_basic_typing: forall (Γ: listctx pty) (e: tm) (τ: hty),
+    Γ ⊢ e ⋮t τ -> ⌊ Γ ⌋* ⊢t e ⋮t ⌊ τ ⌋.
+Proof.
+  all: destruct 1; cbn; subst;
+    eauto using value_has_type, tm_has_type, ctx_erase_lookup.
+  - econstructor.
+    instantiate_atom_listctx.
+    rewrite <- ctx_erase_app_r by my_set_solver.
+    qauto.
+  - rewrite <- H1. econstructor.
+    instantiate_atom_listctx.
+    eapply value_typing_regular_basic_typing in H0.
+    srewrite H1.
+    apply_eq H0. apply ctx_erase_app_r. my_set_solver.
+  - erewrite <- subtyping_preserves_basic_typing; eauto.
+  - econstructor. apply tm_typing_regular_basic_typing. eauto.
+    instantiate_atom_listctx.
+    sinvert H. simpl_Forall2.
+    cbn. eapply_eq tm_typing_regular_basic_typing; eauto.
+    rewrite ctx_erase_app_r by my_set_solver.
+    f_equal. apply tm_typing_regular_wf in H0. sinvert H0. eauto.
+  - econstructor; eauto.
+    apply_eq value_typing_regular_basic_typing; eauto.
+    instantiate_atom_listctx.
+    sinvert H. simpl_Forall2.
+    eapply_eq tm_typing_regular_basic_typing; eauto.
+    rewrite ctx_erase_app_r by my_set_solver.
+    rewrite <- pty_erase_open_eq.
+    f_equal. apply value_typing_regular_wf in H1. sinvert H1. eauto.
+  - econstructor; eauto.
+    sinvert H1. apply subtyping_preserves_basic_typing in H2.
+    cbn in H2. sinvert H2. srewrite H6. eauto.
+    instantiate_atom_listctx.
+    sinvert H. simpl_Forall2.
+    apply_eq tm_typing_regular_basic_typing; eauto.
+    rewrite ctx_erase_app_r by my_set_solver.
+    f_equal.
+  - econstructor; qauto.
+  - econstructor; qauto.
+Qed.
+
 Lemma reduction_tlete:  forall e_x e α β v,
     α ⊧ tlete e_x e ↪*{ β } v <->
     (exists (βx βe: trace) (v_x: value),
       β = βx ++ βe /\ α ⊧ e_x ↪*{ βx } v_x /\ (α ++ βx) ⊧ (e ^t^ v_x) ↪*{ βe } v).
-Admitted.
-
-(* I have proved this lemma in Poirot. *)
-Lemma msubst_open: forall (Γv: env) e (v_x: value) (x: atom),
-    x # (dom Γv ∪ stale e ∪ stale v_x) ->
-    (m{Γv}t) e ^t^ v_x = (m{<[x:=v_x]> Γv}t) (e ^t^ x).
-Admitted.
-
-(** maybe open/close should be a type class *)
-
-Lemma msubst_open_hty: forall (Γv: env) e (v_x: value) (x: atom),
-    x # (dom Γv ∪ stale e ∪ stale v_x) ->
-    (m{Γv}h) e ^h^ v_x = (m{<[x:=v_x]> Γv}h) (e ^h^ x).
-Admitted.
-
-Lemma msubst_hty: forall (Γv: env) T A B, m{Γv}h [:T|A⇒B] = [:T|m{Γv}a A ⇒ m{Γv}pa B].
-Admitted.
-
-Lemma msubst_lete: forall (Γv: env) e_x e, (m{Γv}t (tlete e_x e) = tlete ((m{Γv}t) e_x) ((m{Γv}t) e)).
-Admitted.
-
-Lemma msubst_concat: forall (Γv: env) A1 A2, m{Γv}a (aconcat A1 A2) = (aconcat (m{Γv}a A1) (m{Γv}a A2)).
-Admitted.
-
-Lemma msubst_amlist_typed: forall (Γv: env) B T,
-    amlist_typed ((m{Γv}pa) B) T <-> amlist_typed B T.
-Admitted.
-
-Lemma in_msubst: forall (Γv: env) (A: am) (ρ: pty) (B: list (am * pty)),
-    In (A, ρ) (m{Γv}pa B) <-> exists A' ρ', A = m{Γv}a A' /\ ρ = m{Γv}p ρ' /\ In (A', ρ') B.
-Admitted.
-
-Definition subst4 Γv (x: am * pty * am * pty) :=
-  match x with
-    | (A, ρa, B, ρb) => (m{Γv}a A, m{Γv}p ρa, m{Γv}a B, m{Γv}p ρb)
-  end.
-
-Lemma in_msubst4: forall (Γv: env) (A1: am) (ρ1: pty) (A2: am) (ρ2: pty) (B4: list (am * pty * am * pty)),
-    In (A1, ρ1, A2, ρ2) (List.map (subst4 Γv) B4) ->
-    exists A1' ρ1' A2' ρ2',
-      A1 = m{Γv}a A1' /\ ρ1 = m{Γv}p ρ1' /\ A2 = m{Γv}a A2' /\ ρ2 = m{Γv}p ρ2' /\ In (A1', ρ1', A2', ρ2') B4.
 Admitted.
 
 Lemma am_concat: forall A B α β,
@@ -208,26 +299,42 @@ Proof.
   intros. inversion H. inversion H0; subst; auto. inversion H0.
 Qed.
 
-Lemma ptyR_typed_closed t ρ e :
-  ptyR t ρ e ->
-  ⌊ ρ ⌋ = t /\ ∅ ⊢t e ⋮t ⌊ ρ ⌋ /\ closed_pty ∅ ρ.
+Lemma wf_pty_closed Γ ρ :
+  wf_pty Γ ρ ->
+  closed_pty (ctxdom ⦑ Γ ⦒) ρ.
 Proof.
-  destruct t; simpl; intuition.
-Qed.
-
-Lemma ctxRst_closed_env Γ Γv : ctxRst Γ Γv -> closed_env Γv.
-Proof.
-  unfold closed_env.
-  induction 1.
-  - apply map_Forall_empty.
-  - apply map_Forall_insert_2; eauto.
-    unfold closed_value.
-    change (fv_value v) with (fv_tm v).
-    apply equiv_empty.
-    erewrite <- dom_empty.
-    eapply basic_typing_contains_fv_tm.
-    eapply ptyR_typed_closed.
-    eauto.
+  induction 1; eauto.
+  sinvert IHwf_pty.
+  econstructor.
+  - econstructor; eauto.
+    instantiate_atom_listctx.
+    eapply H4; eauto.
+  - econstructor; eauto.
+    instantiate_atom_listctx.
+    apply H2.
+    intros. repeat specialize_with x.
+    eapply H2; eauto.
+    intros. repeat specialize_with x.
+    eapply H4; eauto.
+  - simpl.
+    repeat apply union_least. eauto. {
+      auto_pose_fv x. repeat specialize_with x. simp_hyps.
+      sinvert H2.
+      rewrite <- open_var_fv_am' in *.
+      rewrite remove_arr_pty_ctx_dom_union in *.
+      rewrite union_mono_l in * by apply remove_arr_pty_ctx_dom_singleton.
+      my_set_solver.
+    }
+    apply union_list_subseteq_forall.
+    setoid_rewrite in_map_iff.
+    intros. simp_hyps. set_fold_not. simpl in *. subst.
+    auto_pose_fv x. repeat specialize_with x. simp_hyps.
+    sinvert H2. sinvert H4.
+    rewrite <- open_var_fv_am' in *.
+    rewrite <- open_var_fv_pty' in *.
+    rewrite remove_arr_pty_ctx_dom_union in *.
+    rewrite union_mono_l in * by apply remove_arr_pty_ctx_dom_singleton.
+    my_set_solver.
 Qed.
 
 Ltac apply_msubst_ind :=
@@ -298,6 +405,41 @@ Ltac apply_msubst_insert :=
   (* TODO: hintdb? *)
   eauto using subst_commute_value, subst_commute_tm, subst_commute_qualifier,
     subst_commute_pty, subst_commute_am, subst_commute_postam.
+
+Lemma pty_erase_msubst_eq ρ Γv :
+  pty_erase ρ = pty_erase (m{Γv}p ρ).
+Proof.
+  msubst_tac.
+  qauto using pty_erase_subst_eq.
+Qed.
+
+Lemma msubst_hty: forall (Γv: env) T A B, m{Γv}h [:T|A⇒B] = [:T|m{Γv}a A ⇒ m{Γv}pa B].
+Admitted.
+
+Lemma msubst_lete: forall (Γv: env) e_x e, (m{Γv}t (tlete e_x e) = tlete ((m{Γv}t) e_x) ((m{Γv}t) e)).
+Admitted.
+
+Lemma msubst_concat: forall (Γv: env) A1 A2, m{Γv}a (aconcat A1 A2) = (aconcat (m{Γv}a A1) (m{Γv}a A2)).
+Admitted.
+
+Lemma msubst_amlist_typed: forall (Γv: env) B T,
+    amlist_typed ((m{Γv}pa) B) T <-> amlist_typed B T.
+Admitted.
+
+Lemma in_msubst: forall (Γv: env) (A: am) (ρ: pty) (B: list (am * pty)),
+    In (A, ρ) (m{Γv}pa B) <-> exists A' ρ', A = m{Γv}a A' /\ ρ = m{Γv}p ρ' /\ In (A', ρ') B.
+Admitted.
+
+Definition subst4 Γv (x: am * pty * am * pty) :=
+  match x with
+    | (A, ρa, B, ρb) => (m{Γv}a A, m{Γv}p ρa, m{Γv}a B, m{Γv}p ρb)
+  end.
+
+Lemma in_msubst4: forall (Γv: env) (A1: am) (ρ1: pty) (A2: am) (ρ2: pty) (B4: list (am * pty * am * pty)),
+    In (A1, ρ1, A2, ρ2) (List.map (subst4 Γv) B4) ->
+    exists A1' ρ1' A2' ρ2',
+      A1 = m{Γv}a A1' /\ ρ1 = m{Γv}p ρ1' /\ A2 = m{Γv}a A2' /\ ρ2 = m{Γv}p ρ2' /\ In (A1', ρ1', A2', ρ2') B4.
+Admitted.
 
 Lemma msubst_fv {T: Type} `{@Stale aset T} : forall (Γv: env) (x: atom) (v_x: value)
                              (f_subst: atom -> value -> T -> T)
@@ -415,13 +557,16 @@ Proof.
   msubst_tac.
   unfold pty_to_rty.
   simpl. f_equal.
-
-  admit.
-  admit.
-
-  repeat f_equal.
-  apply_msubst_insert.
-Admitted.
+  - repeat
+      match goal with
+      | |- context [map_fold pty_subst ?ρ ?m] =>
+          change (map_fold pty_subst ρ m) with (msubst pty_subst m ρ)
+      end.
+    rewrite msubst_insert; eauto using subst_commute_pty.
+    rewrite <- pty_erase_subst_eq. reflexivity.
+  - repeat f_equal.
+    apply_msubst_insert.
+Qed.
 
 Ltac msubst_simp :=
   match goal with
@@ -453,9 +598,66 @@ Ltac msubst_simp :=
   | |- context [ m{ _ }v (vfvar _) ] => rewrite msubst_fvar
   | H: context [ m{ _ }v (vconst _) ] |- _ => rewrite msubst_constant in H
   | |- context [ m{ _ }v (vconst _) ] => rewrite msubst_constant
-  | H: context [ m{ _ }q _ ] |- _ => rewrite msubst_qualifier in H
-  | |- context [ m{ _ }q _ ] => rewrite msubst_qualifier
+  (* | H: context [ m{ _ }q _ ] |- _ => rewrite msubst_qualifier in H *)
+  (* | |- context [ m{ _ }q _ ] => rewrite msubst_qualifier *)
   end; eauto using ctxRst_closed_env.
+
+(** maybe open/close should be a type class *)
+(* I have proved this lemma in Poirot. *)
+Lemma msubst_open: forall (Γv: env) e (v_x: value) (x: atom),
+    closed_env Γv ->
+    closed_value v_x ->
+    map_Forall (fun _ v => lc (treturn v)) Γv ->
+    x ∉ dom Γv ∪ stale e ->
+    (m{Γv}t) e ^t^ v_x = (m{<[x:=v_x]> Γv}t) (e ^t^ x).
+Proof.
+  intros.
+  rewrite msubst_insert; eauto using subst_commute_tm.
+  2 : apply not_elem_of_dom; my_set_solver.
+  revert_all.
+  intros *.
+  msubst_tac.
+  rewrite map_fold_empty. rewrite open_subst_same_tm. auto. my_set_solver.
+  change (map_fold tm_subst ?e ?m) with (msubst tm_subst m e) in *.
+  rewrite msubst_insert; eauto using subst_commute_tm.
+  rewrite subst_commute_tm.
+  rewrite <- H0.
+  rewrite subst_open_tm_closed. reflexivity. eauto.
+  apply map_Forall_insert in H3; eauto. qauto.
+  apply map_Forall_insert in H3; eauto. qauto.
+  my_set_solver.
+  my_set_solver.
+  my_set_solver.
+  my_set_solver.
+Qed.
+
+Lemma msubst_open_hty: forall (Γv: env) e (v_x: value) (x: atom),
+    closed_env Γv ->
+    closed_value v_x ->
+    map_Forall (fun _ v => lc (treturn v)) Γv ->
+    x ∉ dom Γv ∪ stale e ->
+    (m{Γv}h) e ^h^ v_x = (m{<[x:=v_x]> Γv}h) (e ^h^ x).
+Proof.
+  intros.
+  rewrite msubst_insert; eauto using subst_commute_hty.
+  2 : apply not_elem_of_dom; my_set_solver.
+  revert_all.
+  intros *.
+  msubst_tac.
+  rewrite map_fold_empty.
+  rewrite open_subst_same_hty. auto. my_set_solver.
+  change (map_fold hty_subst ?e ?m) with (msubst hty_subst m e) in *.
+  rewrite msubst_insert; eauto using subst_commute_hty.
+  rewrite subst_commute_hty.
+  rewrite <- H0.
+  rewrite subst_open_hty_closed. reflexivity. eauto.
+  apply map_Forall_insert in H3; eauto. qauto.
+  apply map_Forall_insert in H3; eauto. qauto.
+  my_set_solver.
+  my_set_solver.
+  my_set_solver.
+  my_set_solver.
+Qed.
 
 Lemma ptyR_msubst_insert_eq Γv ρ v x u :
   closed_env Γv ->
@@ -468,16 +670,6 @@ Proof.
   rewrite subst_fresh_pty. auto.
   select (p⟦_⟧ _) (fun H => apply ptyR_typed_closed in H).
   simp_hyps. select (closed_pty _ _) (fun H => sinvert H). my_set_solver.
-Qed.
-
-Lemma ctxRst_dom Γ Γv x :
-  ctxRst Γ Γv ->
-  x ∉ ctxdom Γ <-> x ∉ dom Γv.
-Proof.
-  induction 1; simpl; eauto.
-  rewrite ctxdom_app_union.
-  rewrite dom_insert.
-  simpl. my_set_solver.
 Qed.
 
 Lemma ctxRst_ctxfind Γ Γv x ρ :
@@ -500,7 +692,9 @@ Proof.
         (fun H => apply basic_typing_contains_fv_tm in H; simpl in H).
       my_set_solver.
       select (ok_ctx _) (fun H => apply ok_ctx_ok in H; apply ok_post_destruct in H).
-      simp_hyps. apply not_elem_of_dom. eapply ctxRst_dom; eauto.
+      srewrite ctxRst_dom.
+      simp_hyps.
+      apply not_elem_of_dom. eauto.
     }
 
     destruct_or!; simp_hyps.
@@ -516,15 +710,51 @@ Proof.
       eexists. split; eauto. by simplify_map_eq.
 Qed.
 
+Lemma msubst_preserves_basic_typing Γ Γv :
+  ctxRst Γ Γv ->
+  forall Γ' e T,
+    (⌊Γ⌋* ∪ Γ') ⊢t e ⋮t T ->
+    Γ' ⊢t m{Γv}t e ⋮t T.
+Proof.
+  induction 1; intros; eauto.
+  apply_eq H. cbn. apply map_empty_union.
+  rewrite ctx_erase_app in H2.
+  rewrite <- map_union_assoc in H2.
+  apply IHctxRst in H2.
+  apply ptyR_typed_closed in H1. simp_hyps.
+  rewrite msubst_insert; eauto using subst_commute_tm, ctxRst_closed_env.
+  - eapply basic_typing_subst_tm; cycle 1.
+    eapply_eq H2.
+    cbn. rewrite map_union_empty. rewrite insert_empty.
+    rewrite <- insert_union_singleton_l. reflexivity.
+    eapply basic_typing_weaken_value. apply map_empty_subseteq.
+    sinvert H3. apply_eq H6. eauto using pty_erase_msubst_eq.
+  - apply basic_typing_contains_fv_tm in H3. my_set_solver.
+  - sinvert H0; listctx_set_simpl.
+    rewrite ctxRst_dom in H7 by eauto.
+    by apply not_elem_of_dom.
+Qed.
+
+Lemma msubst_preserves_basic_typing_empty Γ Γv :
+  ctxRst Γ Γv ->
+  forall e T,
+    (⌊Γ⌋*) ⊢t e ⋮t T ->
+    ∅ ⊢t m{Γv}t e ⋮t T.
+Proof.
+  intros. eapply msubst_preserves_basic_typing; eauto.
+  rewrite map_union_empty. eauto.
+Qed.
 
 Lemma value_reduction_refl: forall α β (v1: value) v2, α ⊧ v1 ↪*{ β} v2 -> v2 = v1 /\ β = [].
-Admitted.
+Proof.
+  intros * H.
+  sinvert H; easy.
+Qed.
 
 Ltac reduction_simp :=
   match goal with
-  | H: _ ⊧ (treturn _) ↪*{ _ } _  |- _ => apply value_reduction_refl in H;
-                                        destruct H as (Htmp1 & Htmp2);
-                                        subst; try rewrite Htmp1; try clear Htmp1; try clear Htmp2
+  | H: _ ⊧ (treturn _) ↪*{ _ } _  |- _ =>
+      apply value_reduction_refl in H; simp_hyps; simplify_eq
   end.
 
 Lemma denotation_application_base_arg:
@@ -532,7 +762,22 @@ Lemma denotation_application_base_arg:
     Tb = b ->
     (forall(v: value), p⟦ {v:b|ϕ} ⟧ v -> ⟦ [:T | A ^a^ v ⇒ B ^pa^ v ] ⟧ (e ^t^ v)) ->
     p⟦ -: {v:b|ϕ} ⤑[:T|A⇒B] ⟧ (vlam Tb e).
-Admitted.
+Proof.
+  intros.
+  cbn.
+  split; eauto. split. admit. split. admit.
+  intros.
+  apply H0 in H2.
+  hnf in H2.
+  cbn in H2.
+  simp_hyps.
+  feed specialize H7.
+  admit.
+  edestruct H7; eauto.
+  eapply_eq H4.
+  admit.
+  simp_hyps.
+
 
 Lemma denotation_application_arr_arg:
   forall ρx (Tx: ty) Ax Bx T A B Te e,
@@ -565,26 +810,37 @@ Lemma reduction_matchb_false:  forall e1 e2 α β v,
     α ⊧ tmatchb false e1 e2 ↪*{ β} v <-> lc e1 /\ α ⊧ e2 ↪*{ β} v.
 Admitted.
 
-Lemma lc_am_dot: lc_am ∘.
-Admitted.
-
-Lemma am_fv_dot_empty: am_fv ∘ = ∅.
-Admitted.
+Lemma pty_to_rty_preserves_closed: forall (ρ: pty) d,
+    closed_pty d ρ -> closed_hty d (pty_to_rty ρ).
+Proof.
+  inversion 1.
+  repeat econstructor; try solve [hnf; qauto]. qsimpl.
+  cbn. repeat my_set_solver.
+Qed.
 
 Lemma denotation_value_pure: forall (ρ: pty) (v: value), p⟦ ρ ⟧ v <-> ⟦pty_to_rty ρ ⟧ v.
 Proof.
-  unfold pty_to_rty; split; intros.
-  - split. admit. split. admit.
+  split; simpl; intros.
+  - dup_hyp H (fun H => apply ptyR_typed_closed in H).
+    simp_hyps.
+    split; simpl; eauto. split; eauto using pty_to_rty_preserves_closed.
     intros Hamlist α β v' Hα Hstepv. reduction_simp.
     exists aϵ, ρ. split. unfold In. left; auto. split; auto. repeat constructor; auto.
   - destruct H as (Ht & Hclose & H).
-    assert (amlist_typed [(aϵ, ρ)] ⌊ρ⌋) as Hamlist. { admit. }
+    cbn in *.
+    assert (amlist_typed [(aϵ, ρ)] ⌊ρ⌋) as Hamlist. {
+      clear. hnf. qauto.
+    }
     specialize (H Hamlist [] [] v).
-    assert (closed_am ∅ (astar ∘) ∧ repeat_tr (a⟦∘⟧) []) as H1.
-    { split; auto. repeat constructor; simpl; auto. apply lc_am_dot. rewrite am_fv_dot_empty; auto. constructor. }
-    assert ([] ⊧ v ↪*{ [] } v) as Hstepv. constructor. admit.
+    assert (closed_am ∅ (astar ∘) ∧ repeat_tr (a⟦∘⟧) []) as H1. {
+      split; auto. repeat constructor; simpl; auto. econstructor.
+    }
+    assert ([] ⊧ v ↪*{ [] } v) as Hstepv. {
+      econstructor.
+      eauto using basic_typing_regular_tm.
+    }
     specialize (H H1 Hstepv). mydestr. apply in_singleton in H. mydestr; subst; auto.
-Admitted.
+Qed.
 
 Lemma closed_bool_typed_value: forall v, ∅ ⊢t v ⋮v TBool -> v = true \/ v = false.
 Proof.
@@ -607,9 +863,6 @@ Theorem fundamental: forall (Γ: listctx pty) (e: tm) (τ: hty),
     forall Γv, ctxRst Γ Γv -> ⟦ msubst hty_subst Γv τ ⟧ (msubst tm_subst Γv e).
 Proof.
   apply (term_type_check_rec
-           (* NOTE: should this be the denotation of [pty]? *)
-           (* (fun Γ (v: value) ρ _ => *)
-           (*    forall Γv, ctxRst Γ Γv -> ⟦ m{Γv}h (pty_to_rty ρ) ⟧ (m{Γv}v v)) *)
            (fun Γ (v: value) ρ _ =>
               forall Γv, ctxRst Γ Γv -> p⟦ m{Γv}p ρ ⟧ (m{Γv}v v))
            (fun Γ e (τ: hty) _ =>
@@ -619,59 +872,158 @@ Proof.
   - intros Γ c HWF Γv HΓv. repeat msubst_simp.
     assert ((m{Γv}p) (mk_eq_constant c) = (mk_eq_constant c)) as Htmp. {
       unfold mk_eq_constant, mk_q_bvar_eq_val.
-      repeat (msubst_simp; simpl).
+      repeat (simpl; msubst_simp).
+      rewrite msubst_qualifier; eauto using ctxRst_closed_env.
+      repeat (simpl; msubst_simp).
     }
     rewrite Htmp; clear Htmp.
     simpl.
     repeat split; try solve [repeat econstructor].
     simpl. set_solver.
     intros. unfold bpropR. simpl.
-    specialize (H []). apply multi_step_value in H.
-    qauto.
+    specialize (H []). apply value_reduction_refl in H.
+    simp_hyps. eauto.
 
   (* [TVar] *)
-  - intros Γ x ρ Hfind Γv HΓv. repeat msubst_simp.
+  - intros Γ x ρ Hwf Hfind Γv HΓv. repeat msubst_simp.
     eapply ctxRst_ctxfind in HΓv; eauto.
     qauto.
 
   (* [TLam] *)
-  - intros Γ Tx ρ e T A B L HWF _ HDe Γv HΓv. repeat msubst_simp.
+  - intros Γ Tx ρ e T A B L HWF Ht HDe He Γv HΓv. repeat msubst_simp.
     auto_pose_fv x. repeat specialize_with x.
     destruct ρ.
-    + repeat msubst_simp. apply denotation_application_base_arg. admit.
-      intros v_x Hv_x. assert (ctxRst (Γ ++ [(x, {v:B0|ϕ})]) (<[x := v_x]> Γv)) as HΓv'. admit.
+    + repeat msubst_simp. apply denotation_application_base_arg. eauto.
+      intros v_x Hv_x.
+      assert (ctxRst (Γ ++ [(x, {v:B0|ϕ})]) (<[x := v_x]> Γv)) as HΓv'. {
+        econstructor; eauto.
+        econstructor; eauto using ctxRst_ok_ctx.
+        sinvert HWF. sinvert H4. eauto.
+        my_set_solver.
+        msubst_simp.
+      }
       specialize (HDe _ HΓv').
-      rewrite <- msubst_open in HDe. 2: { admit. } rewrite <- msubst_open_hty in HDe. 2: { admit. }
-      repeat msubst_simp. auto.
-    + repeat msubst_simp. apply denotation_application_arr_arg. admit.
-      intros v_x Hv_x. assert (ctxRst (Γ ++ [(x, -:ρ⤑[:T0|pre⇒post] )]) (<[x := v_x]> Γv)) as HΓv'. admit.
+      rewrite <- msubst_open in HDe;
+        eauto using ctxRst_closed_env, ctxRst_lc, ptyR_closed_value.
+      2 : {
+        simpl in *. srewrite ctxRst_dom. my_set_solver.
+      }
+      rewrite <- msubst_open_hty in HDe.
+      2: {
+        simpl in *. srewrite ctxRst_dom.
+        simp_hyps.
+        apply basic_typing_contains_fv_tm in H2. simpl in *.
+        my_set_solver.
+      }
+      repeat msubst_simp.
+    + repeat msubst_simp. apply denotation_application_arr_arg.
+
+      (* TODO: Lemma *)
+      cbv in He. fold pty_erase in He. subst.
+      f_equal.
+      unfold erase. unfold pty_erase_.
+      clear - HΓv.
+      induction ρ.
+      repeat msubst_simp.
+      repeat msubst_simp.
+      simpl. f_equal. eauto.
+
+      intros v_x Hv_x.
+      assert (ctxRst (Γ ++ [(x, -:ρ⤑[:T0|pre⇒post] )]) (<[x := v_x]> Γv)) as HΓv'. {
+        econstructor; eauto.
+        econstructor; eauto using ctxRst_ok_ctx.
+        sinvert HWF.
+        apply wf_pty_closed. eauto.
+        my_set_solver.
+        msubst_simp.
+      }
       specialize (HDe _ HΓv').
       rewrite <- msubst_open in HDe.
-      2: { admit. }
-      assert ((m{<[x:=v_x]> Γv}h) ([:T|A⇒B] ^h^ x) = m{Γv}h [:T|A⇒B]) as Htmp3. admit. rewrite Htmp3 in HDe.
-      repeat msubst_simp. auto.
+      all: eauto using ctxRst_closed_env, ctxRst_lc.
+      2: {
+        apply ptyR_typed_closed in Hv_x. simp_hyps.
+        apply basic_typing_contains_fv_tm in H1.
+        my_set_solver.
+      }
+      2: {
+        simpl in *. srewrite ctxRst_dom.
+        simp_hyps.
+        apply basic_typing_contains_fv_tm in H2. simpl in *.
+        my_set_solver.
+      }
+      assert ((m{<[x:=v_x]> Γv}h) ([:T|A⇒B] ^h^ x) = m{Γv}h [:T|A⇒B]) as Htmp3. {
+        (* rewrite <- msubst_open_hty. *)
+        admit.
+      }
+      rewrite Htmp3 in HDe.
+      repeat msubst_simp.
 
-  - intros Γ Tx ρ e T A B L HWF _ HDe Γv HΓv. repeat msubst_simp. rewrite <- denotation_value_pure.
+  (* [TLamFix] *)
+  - intros Γ Tx ρ e T A B L HWF Hlam HDe Γv He HΓv. repeat msubst_simp.
     auto_pose_fv f. repeat specialize_with f. admit.
-  - intros Γ v ρ _ HDv Γv HΓv. specialize (HDv _ HΓv). repeat msubst_simp. auto.
+
+  (* [TValue] *)
+  - intros Γ v ρ _ HDv Γv HΓv. specialize (HDv _ HΓv).
+    repeat msubst_simp. rewrite <- denotation_value_pure. auto.
+
+  (* [TSub] *)
   - intros Γ e τ1 τ2 HWFτ2 _ HDτ1 Hsub Γv HΓv. specialize (HDτ1 _ HΓv). apply Hsub in HDτ1; auto.
-  - intros Γ e_x e Tx A T Bx_ρx BxB_ρ Bx_ρx_B_ρ L HWFBρ HTe_x HDe_x Hin1 Hin2 _ He Γv HΓv.
-    auto_pose_fv x. repeat specialize_with x. repeat msubst_simp.
-    split. admit. split. admit.
+
+  (* [TLetE] *)
+  - intros Γ e_x e Tx A T Bx_ρx BxB_ρ Bx_ρx_B_ρ L HWFBρ HTe_x HDe_x Hin1 Hin2 Ht He Γv HΓv.
+    split; [| split]. {
+      eapply msubst_preserves_basic_typing_empty; eauto.
+      econstructor. eauto using tm_typing_regular_basic_typing.
+      instantiate_atom_listctx.
+      admit.
+    } {
+      (* [hty] *)
+      (* Γ |-WF τ -> closed Γ τ -> closed ∅ (m{Γv} τ) *)
+      admit.
+    }
+    repeat msubst_simp.
     intros HBtyped α β v HDα Hstepv.
-    rewrite reduction_tlete in Hstepv. destruct Hstepv as (βx & βe & v_x & Htmp & Hstepv_x & Hstepv). subst.
-    rewrite msubst_open with (x:=x) in Hstepv. 2: { admit. }
+    rewrite reduction_tlete in Hstepv. destruct Hstepv as (βx & βe & v_x & Htmp & Hstepv_x & Hstepv).
+    auto_pose_fv x. repeat specialize_with x.
+    rewrite msubst_open with (x:=x) in Hstepv.
+    2: {
+      simpl in *.
+      rewrite ctxRst_dom in H by eauto.
+      my_set_solver.
+    }
     specialize (HDe_x _ HΓv). repeat msubst_simp.
     destruct HDe_x as (Hte_x & Hclosede_x & HDe_x).
-    assert (amlist_typed ((m{Γv}pa) Bx_ρx) Tx) as HH1. { rewrite msubst_amlist_typed. admit. }
+    assert (amlist_typed ((m{Γv}pa) Bx_ρx) Tx) as HH1. {
+      clear - Hclosede_x.
+      sinvert Hclosede_x.
+      sinvert H.
+      eauto.
+    }
+    block_hyp Hin1. block_hyp Hin2.
     specialize (HDe_x HH1 _ _ _ HDα Hstepv_x).
     destruct HDe_x as (Bxi' & ρxi' & HinBx_ρx & Hβx & Hv_x).
-    apply in_msubst in HinBx_ρx. destruct HinBx_ρx as (Bxi & ρxi & Htmp0 & Htmp1 & HinBx_ρx); subst.
-    apply Hin1 in HinBx_ρx. destruct HinBx_ρx as (Bi & ρi & Hin). clear Hin1.
-    assert (ctxRst (Γ ++ [(x, ρxi)]) (<[x:=v_x]> Γv)) as HH2. { constructor; auto. admit. }
+    apply in_msubst in HinBx_ρx. destruct HinBx_ρx as (Bxi & ρxi & Htmp0 & Htmp1 & HinBx_ρx). subst.
+    (* apply Hin1 in HinBx_ρx. destruct HinBx_ρx as (Bi & ρi & Hin). clear Hin1. *)
+    assert (ctxRst (Γ ++ [(x, ρxi)]) (<[x:=v_x]> Γv)) as HH2. {
+      constructor; auto.
+      econstructor. eauto using ctxRst_ok_ctx.
+      (* well-typed -> well-formed *)
+      admit.
+      my_set_solver.
+    }
+    assert (exists Bi ρi, In (Bxi, ρxi, Bi, ρi) Bx_ρx_B_ρ) as Hin. {
+      unblock_hyps. subst.
+      clear - HinBx_ρx.
+      apply in_map_iff in HinBx_ρx. simp_hyps.
+      eauto.
+    }
+    destruct Hin as (Bi & ρi & Hin).
     specialize (He _ _ _ _ Hin (<[ x := v_x]> Γv) HH2). repeat msubst_simp.
     destruct He as (Hte & Hclosede & He).
-    assert (amlist_typed ((m{<[x:=v_x]> Γv}pa) [(Bi, ρi)]) T) as HH3. { rewrite msubst_amlist_typed. admit. }
+    assert (amlist_typed ((m{<[x:=v_x]> Γv}pa) [(Bi, ρi)]) T) as HH3. {
+      rewrite msubst_amlist_typed.
+      admit.
+    }
     specialize (He HH3 (α ++ βx) βe v).
     assert (x ∉ stale Bxi). admit.
     assert ((a⟦(m{<[x:=v_x]> Γv}a) (aconcat A Bxi)⟧) (α ++ βx)) as Hconcat.
@@ -680,17 +1032,24 @@ Proof.
     specialize (He Hconcat Hstepv). destruct He as (Bi'' & ρi'' & Hini & Hβe & Hv).
     apply in_msubst in Hini. destruct Hini as (Bi' & ρi' & Htmp0 & Htmp1 & Hini); subst.
     apply in_singleton in Hini. mydestr; subst.
-    assert (In ((aconcat Bxi Bi), ρi) BxB_ρ) as Hinii. { apply Hin2. eauto. }
+    assert (In ((aconcat Bxi Bi), ρi) BxB_ρ) as Hinii. {
+      unblock_hyps. subst.
+      apply in_map_iff.
+      repeat eexists. 2: eauto.
+      eauto.
+    }
     exists (m{<[x:=v_x]> Γv}a (aconcat Bxi Bi)), (m{<[x:=v_x]> Γv}p ρi).
     repeat split; auto.
     + rewrite in_msubst. exists (aconcat Bxi Bi), ρi. repeat split; auto.
       * rewrite msubst_fv; auto. admit.
       * rewrite msubst_fv; auto. admit.
     + repeat msubst_simp. apply am_concat; auto. rewrite am_denotation_fv; auto.
+
   - intros Γ v1 v2 e ρ Tx A T Bx_ρx BxB_ρ Bx_ρx_B_ρ L HWF _ HDv2 _ HDv1 Hin1 Hin2 _ He Γv HΓv.
     auto_pose_fv x. repeat specialize_with x. repeat msubst_simp.
     specialize (HDv1 _ HΓv). specialize (HDv2 _ HΓv). repeat msubst_simp.
     rewrite <- denotation_value_pure in HDv1. rewrite <- denotation_value_pure in HDv2. admit.
+
   - intros Γ op v2 e ρ A ϕx T Aop' Bi ρi L HAop' HWF Hbuiltin _ HDv2 _ He Γv HΓv.
     auto_pose_fv x. repeat specialize_with x. specialize (HDv2 _ HΓv).
     split. admit. split. admit. repeat msubst_simp.
@@ -719,6 +1078,7 @@ Proof.
       assert (y1 = m{Γv}a Bi /\ y2 = m{Γv}p ρi) as Htmp4. admit. mydestr; subst.
       split; auto. repeat msubst_simp. admit.
     + admit.
+
   - intros Γ v e1 e2 τ HWFτ _ HDv _ HDe1 Hte2 Γv HΓv.
     specialize (HDv _ HΓv). specialize (HDe1 _ HΓv). repeat msubst_simp. rewrite <- denotation_value_pure in HDv.
     assert (((m{Γv}v) v) = true) as Htmp. admit. rewrite Htmp in HDv. rewrite Htmp. clear Htmp.
